Mica/Verifier/BoundedQuantifier.lean
@@ -184,7 +184,7 @@ def intrinsic (name : String) (path : String) : Verifier.Intrinsic where
   retTy := .bool
   spec :=
     { args := ["lo", "hi", "body"]
-      pred := .assert .false_ (.ret ("ret", .ret ())) }
+      pred := .assert .false_ (.ret ⟨"ret", .ret ()⟩) }
   typing := Verifier.monoTyping .three
   folSym := none
   axioms := []
